<?xml version="1.0"?>
<rdf:RDF xmlns="https://w3id.org/OPLaX/"
     xml:base="https://w3id.org/OPLaX/"
     xmlns:dc="http://purl.org/dc/elements/1.1/"
     xmlns:owl="http://www.w3.org/2002/07/owl#"
     xmlns:rdf="http://www.w3.org/1999/02/22-rdf-syntax-ns#"
     xmlns:xml="http://www.w3.org/XML/1998/namespace"
     xmlns:xsd="http://www.w3.org/2001/XMLSchema#"
     xmlns:rdfs="http://www.w3.org/2000/01/rdf-schema#"
     xmlns:oplax="https://w3id.org/OPLaX/">
    <owl:Ontology rdf:about="https://w3id.org/OPLaX/">
        <dc:creator>Christian Colonna</dc:creator>
        <dc:creator>Luigi Asprino</dc:creator>
        <dc:creator>Valentina Carriero</dc:creator>
        <dc:creator>Valentina Presutti</dc:creator>
        <rdfs:comment xml:lang="en">This is the extended version of the OPLa ontology, which includes: (i) annotation properties from the original OPLa ontology (Pascal Hitzler et al., Towards a simple but useful Ontology Design Pattern Representation Language, WOP 2017 - https://github.com/cogan-shimizu/Extended-OPLa/blob/master/oplacore.owl); (ii) annotation properties from the Content Pattern annotation schema (http://www.ontologydesignpatterns.org/schemas/cpannotationschema.owl) used in the ODP Portal (http://www.ontologydesignpatterns.org/); (iii) additional annotation properties for addressing the instance level (an instance of a pattern) and the conceptual component level (an abstract conceptual component grouping different patterns addressing it).</rdfs:comment>
        <rdfs:label xml:lang="en">OPLaX (Ontology Pattern Language eXtended) ontology</rdfs:label>
        <owl:versionInfo xml:lang="en">0.0.2</owl:versionInfo>
    </owl:Ontology>
    


    <!-- 
    ///////////////////////////////////////////////////////////////////////////////////////
    //
    // Annotation properties
    //
    ///////////////////////////////////////////////////////////////////////////////////////
     -->

    


    <!-- http://purl.org/dc/elements/1.1/creator -->

    <owl:AnnotationProperty rdf:about="http://purl.org/dc/elements/1.1/creator"/>
    


    <!-- https://w3id.org/OPLaX/componentOfPattern -->

    <owl:AnnotationProperty rdf:about="https://w3id.org/OPLaX/componentOfPattern">
        <rdfs:comment xml:lang="en">This property relates a Pattern to the Pattern it is a component of.</rdfs:comment>
        <rdfs:label xml:lang="en">component of pattern</rdfs:label>
        <rdfs:subPropertyOf rdf:resource="https://w3id.org/OPLaX/hasRelatedPattern"/>
        <rdfs:range rdf:resource="https://w3id.org/OPLaX/Pattern"/>
        <rdfs:domain rdf:resource="https://w3id.org/OPLaX/Pattern"/>
    </owl:AnnotationProperty>
    


    <!-- https://w3id.org/OPLaX/derivedFromModule -->

    <owl:AnnotationProperty rdf:about="https://w3id.org/OPLaX/derivedFromModule">
        <rdfs:comment xml:lang="en">This property relates a Module to the Module it is a derived from.</rdfs:comment>
        <rdfs:label xml:lang="en">derived from module</rdfs:label>
        <rdfs:subPropertyOf rdf:resource="https://w3id.org/OPLaX/hasRelatedModule"/>
        <rdfs:range rdf:resource="https://w3id.org/OPLaX/Module"/>
        <rdfs:domain rdf:resource="https://w3id.org/OPLaX/Module"/>
        <owl:equivalentProperty rdf:resource="http://ontologydesignpatterns.org/opla-core/derivedFromModule"/>
    </owl:AnnotationProperty>
    

    <!-- https://w3id.org/OPLaX/derivedFromPattern -->

    <owl:AnnotationProperty rdf:about="https://w3id.org/OPLaX/derivedFromPattern">
        <rdfs:comment xml:lang="en">This property relates a Pattern to the Pattern it is a derived from.</rdfs:comment>
        <rdfs:label xml:lang="en">derived from pattern</rdfs:label>
        <rdfs:subPropertyOf rdf:resource="https://w3id.org/OPLaX/hasRelatedPattern"/>
        <rdfs:range rdf:resource="https://w3id.org/OPLaX/Pattern"/>
        <rdfs:domain rdf:resource="https://w3id.org/OPLaX/Pattern"/>
        <owl:equivalentProperty rdf:resource="http://ontologydesignpatterns.org/opla-core/derivedFromPattern"/>
    </owl:AnnotationProperty>
    


    <!-- https://w3id.org/OPLaX/description -->

    <owl:AnnotationProperty rdf:about="https://w3id.org/OPLaX/description">
        <rdfs:comment xml:lang="en">This property relates a Conceptual Component to its description.</rdfs:comment>
        <rdfs:label xml:lang="en">description</rdfs:label>
        <rdfs:range rdf:resource="http://www.w3.org/2001/XMLSchema#string"/>
        <rdfs:domain rdf:resource="http://www.w3.org/2002/07/owl#Thing"/>
    </owl:AnnotationProperty>
    


    <!-- https://w3id.org/OPLaX/extractedFrom -->

    <owl:AnnotationProperty rdf:about="https://w3id.org/OPLaX/extractedFrom">
        <rdfs:comment xml:lang="en">This property relates an Ontological Collection to a possible reference ontology which the annotated Ontological Collection was extracted from (i.e. the reference ontology that the ontology elements have been deeply or partially cloned by).</rdfs:comment>
        <rdfs:label xml:lang="en">extracted from</rdfs:label>
        <rdfs:range rdf:resource="https://w3id.org/OPLaX/OntologicalCollection"/>
        <rdfs:domain rdf:resource="https://w3id.org/OPLaX/OntologicalCollection"/>
        <owl:equivalentProperty rdf:resource="http://www.ontologydesignpatterns.org/schemas/cpannotationschema.owl#extractedFrom"/>
    </owl:AnnotationProperty>
    


    <!-- https://w3id.org/OPLaX/generalizationOfConceptualComponent -->

    <owl:AnnotationProperty rdf:about="https://w3id.org/OPLaX/generalizationOfConceptualComponent">
        <rdfs:comment xml:lang="en">This property relates a Conceptual Component to the Conceptual Component it is a generalization of.</rdfs:comment>
        <rdfs:label xml:lang="en">generalization of conceptual component</rdfs:label>
        <rdfs:subPropertyOf rdf:resource="https://w3id.org/OPLaX/hasRelatedConceptualComponent"/>
        <rdfs:range rdf:resource="https://w3id.org/OPLaX/ConceptualComponent"/>
        <rdfs:domain rdf:resource="https://w3id.org/OPLaX/ConceptualComponent"/>
    </owl:AnnotationProperty>
    


    <!-- https://w3id.org/OPLaX/generalizationOfModule -->

    <owl:AnnotationProperty rdf:about="https://w3id.org/OPLaX/generalizationOfModule">
        <rdfs:comment xml:lang="en">This property relates a Module to the Module it is a generalization of.</rdfs:comment>
        <rdfs:label xml:lang="en">generalization of module</rdfs:label>
        <rdfs:subPropertyOf rdf:resource="https://w3id.org/OPLaX/hasRelatedModule"/>
        <rdfs:range rdf:resource="https://w3id.org/OPLaX/Module"/>
        <rdfs:domain rdf:resource="https://w3id.org/OPLaX/Module"/>
        <owl:equivalentProperty rdf:resource="http://ontologydesignpatterns.org/opla-core/generalizationOfModule"/>
    </owl:AnnotationProperty>
    


    <!-- https://w3id.org/OPLaX/generalizationOfPattern -->

    <owl:AnnotationProperty rdf:about="https://w3id.org/OPLaX/generalizationOfPattern">
        <rdfs:comment xml:lang="en">This property relates a Pattern to the Pattern it is a generalization of.</rdfs:comment>
        <rdfs:label xml:lang="en">generalization of pattern</rdfs:label>
        <rdfs:subPropertyOf rdf:resource="https://w3id.org/OPLaX/hasRelatedPattern"/>
        <rdfs:range rdf:resource="https://w3id.org/OPLaX/Pattern"/>
        <rdfs:domain rdf:resource="https://w3id.org/OPLaX/Pattern"/>
        <owl:equivalentProperty rdf:resource="http://ontologydesignpatterns.org/opla-core/generalizationOfPattern"/>
    </owl:AnnotationProperty>
    


    <!-- https://w3id.org/OPLaX/hasCompetencyQuestion -->

    <owl:AnnotationProperty rdf:about="https://w3id.org/OPLaX/hasCompetencyQuestion">
        <rdfs:comment xml:lang="en">This property relates an Ontological Collection or a Conceptual Component to an addressed Competency Question (expressed in natural language) that can be evaluated against them.</rdfs:comment>
        <rdfs:label xml:lang="en">has competency question</rdfs:label>
        <rdfs:range rdf:resource="http://www.w3.org/2001/XMLSchema#string"/>
        <rdfs:domain rdf:resource="http://www.w3.org/2002/07/owl#Thing"/>
        <owl:equivalentProperty rdf:resource="http://www.ontologydesignpatterns.org/schemas/cpannotationschema.owl#hasCompetencyQuestion"/>
    </owl:AnnotationProperty>
    


    <!-- https://w3id.org/OPLaX/hasDomain -->

    <owl:AnnotationProperty rdf:about="https://w3id.org/OPLaX/hasDomain">
        <rdfs:comment xml:lang="en">This property relates an Ontological Collection or a Conceptual Component to their domain (e.g. multimedia, time).</rdfs:comment>
        <rdfs:label xml:lang="en">has domain</rdfs:label>
        <rdfs:range rdf:resource="https://w3id.org/OPLaX/Domain"/>
        <rdfs:domain rdf:resource="http://www.w3.org/2002/07/owl#Thing"/>
    </owl:AnnotationProperty>
    


    <!-- https://w3id.org/OPLaX/hasRelatedConceptualComponent -->

    <owl:AnnotationProperty rdf:about="https://w3id.org/OPLaX/hasRelatedConceptualComponent">
        <rdfs:comment xml:lang="en">This property relates a Conceptual Component to another Conceptual Component.</rdfs:comment>
        <rdfs:label xml:lang="en">has related conceptual component</rdfs:label>
        <rdfs:range rdf:resource="https://w3id.org/OPLaX/ConceptualComponent"/>
        <rdfs:domain rdf:resource="https://w3id.org/OPLaX/ConceptualComponent"/>
    </owl:AnnotationProperty>
    


    <!-- https://w3id.org/OPLaX/hasRelatedModule -->

    <owl:AnnotationProperty rdf:about="https://w3id.org/OPLaX/hasRelatedModule">
        <rdfs:comment xml:lang="en">This property relates a Module to another Module. It does not need to be derived from a module, they simply share the same intent.</rdfs:comment>
        <rdfs:label xml:lang="en">has related module</rdfs:label>
        <rdfs:range rdf:resource="https://w3id.org/OPLaX/Module"/>
        <rdfs:domain rdf:resource="https://w3id.org/OPLaX/Module"/>
        <owl:equivalentProperty rdf:resource="http://ontologydesignpatterns.org/opla-core/hasRelatedModule"/>
    </owl:AnnotationProperty>
    


    <!-- https://w3id.org/OPLaX/hasRelatedPattern -->

    <owl:AnnotationProperty rdf:about="https://w3id.org/OPLaX/hasRelatedPattern">
        <rdfs:comment xml:lang="en">This property relates a Module to another Module. It does not need to be derived from a module, they simply share the same intent.</rdfs:comment>
        <rdfs:label xml:lang="en">has related pattern</rdfs:label>
        <rdfs:range rdf:resource="https://w3id.org/OPLaX/Pattern"/>
        <rdfs:domain rdf:resource="https://w3id.org/OPLaX/Pattern"/>
        <owl:equivalentProperty rdf:resource="http://ontologydesignpatterns.org/opla-core/hasRelatedPattern"/>
    </owl:AnnotationProperty>
    


    <!-- https://w3id.org/OPLaX/implementsConceptualComponent -->

    <owl:AnnotationProperty rdf:about="https://w3id.org/OPLaX/implementsConceptualComponent">
        <rdfs:comment xml:lang="en">This property relates a Pattern to the Conceptual Component it implements.</rdfs:comment>
        <rdfs:label xml:lang="en">implements conceptual component</rdfs:label>
        <rdfs:range rdf:resource="https://w3id.org/OPLaX/ConceptualComponent"/>
        <rdfs:domain rdf:resource="https://w3id.org/OPLaX/Pattern"/>
    </owl:AnnotationProperty>
    


    <!-- https://w3id.org/OPLaX/isMemberOfPatternInstance -->

    <owl:AnnotationProperty rdf:about="https://w3id.org/OPLaX/isMemberOfPatternInstance">
        <rdfs:comment xml:lang="en">This property relates an Ontological Entity to the Pattern Instance it is member of.</rdfs:comment>
        <rdfs:label xml:lang="en">is member of pattern instance</rdfs:label>
        <rdfs:range rdf:resource="https://w3id.org/OPLaX/PatternInstance"/>
        <rdfs:domain rdf:resource="https://w3id.org/OPLaX/OntologicalEntity"/>
    </owl:AnnotationProperty>
    


    <!-- https://w3id.org/OPLaX/isNativeTo -->

    <owl:AnnotationProperty rdf:about="https://w3id.org/OPLaX/isNativeTo">
        <rdfs:comment xml:lang="en">This property relates an Ontological Entity or a Module to an Ontological Collection it is native to.</rdfs:comment>
        <rdfs:label xml:lang="en">is native to</rdfs:label>
        <rdfs:range rdf:resource="https://w3id.org/OPLaX/OntologicalCollection"/>
        <rdfs:domain rdf:resource="http://www.w3.org/2002/07/owl#Thing"/>
        <owl:equivalentProperty rdf:resource="http://ontologydesignpatterns.org/opla-core/isNativeTo"/>
    </owl:AnnotationProperty>
    


    <!-- https://w3id.org/OPLaX/isPatternInstanceOf -->

    <owl:AnnotationProperty rdf:about="https://w3id.org/OPLaX/isPatternInstanceOf">
        <rdfs:comment xml:lang="en">This property relates a Pattern Instance to the Pattern it instantiates.</rdfs:comment>
        <rdfs:label xml:lang="en">is pattern instance of</rdfs:label>
        <rdfs:range rdf:resource="https://w3id.org/OPLaX/Pattern"/>
        <rdfs:domain rdf:resource="https://w3id.org/OPLaX/PatternInstance"/>
    </owl:AnnotationProperty>
    


    <!-- https://w3id.org/OPLaX/name -->

    <owl:AnnotationProperty rdf:about="https://w3id.org/OPLaX/name">
        <rdfs:comment xml:lang="en">This property relates a Conceptual Component or an Ontological Collection to their name.</rdfs:comment>
        <rdfs:label xml:lang="en">name</rdfs:label>
        <rdfs:range rdf:resource="http://www.w3.org/2001/XMLSchema#string"/>
        <rdfs:domain rdf:resource="http://www.w3.org/2002/07/owl#Thing"/>
    </owl:AnnotationProperty>
    


    <!-- https://w3id.org/OPLaX/ofExternalType -->

    <owl:AnnotationProperty rdf:about="https://w3id.org/OPLaX/ofExternalType">
        <rdfs:comment xml:lang="en">This property indicates that another pattern may hook into this entity. For example, a hook might indicate that the pattern developer acknowledges a certain concept is out of scope of the particular pattern.</rdfs:comment>
        <rdfs:label xml:lang="en">of external type</rdfs:label>
        <owl:equivalentProperty rdf:resource="http://ontologydesignpatterns.org/opla-core/ofExternalType"/>
    </owl:AnnotationProperty>
    


    <!-- https://w3id.org/OPLaX/reengineeredFrom -->

    <owl:AnnotationProperty rdf:about="https://w3id.org/OPLaX/reengineeredFrom">
        <rdfs:comment xml:lang="en">This property relates an Ontological Collection to a concept schema, page, or anything else from which the annotated Ontological Collection was reengineered. If the source does not have any URI e.g., a printed book, this property value should provide information as precise as possible in order to identify the source. This property is alternative to the extractedFrom property because it is used when the pattern come from a concept schema which is not an owl ontology.</rdfs:comment>
        <rdfs:label xml:lang="en">reengineered from</rdfs:label>
        <rdfs:range rdf:resource="http://www.w3.org/2002/07/owl#Thing"/>
        <rdfs:domain rdf:resource="https://w3id.org/OPLaX/OntologicalCollection"/>
        <owl:equivalentProperty rdf:resource="http://www.ontologydesignpatterns.org/schemas/cpannotationschema.owl#reengineeredFrom"/>
    </owl:AnnotationProperty>
    


    <!-- https://w3id.org/OPLaX/reusesAsTemplate -->

    <owl:AnnotationProperty rdf:about="https://w3id.org/OPLaX/reusesAsTemplate">
        <rdfs:comment xml:lang="en">This property relates an Ontological Collection to another Ontological Collection that is reused as template.</rdfs:comment>
        <rdfs:label xml:lang="en">reuses as template</rdfs:label>
        <rdfs:range rdf:resource="https://w3id.org/OPLaX/OntologicalCollection"/>
        <rdfs:domain rdf:resource="https://w3id.org/OPLaX/OntologicalCollection"/>
        <owl:equivalentProperty rdf:resource="http://ontologydesignpatterns.org/opla-core/reusesAsTemplate"/>
    </owl:AnnotationProperty>
    


    <!-- https://w3id.org/OPLaX/specializationOfConceptualComponent -->

    <owl:AnnotationProperty rdf:about="https://w3id.org/OPLaX/specializationOfConceptualComponent">
        <rdfs:comment xml:lang="en">This property relates a Conceptual Component to the Conceptual Component it is a specialization of.</rdfs:comment>
        <rdfs:label xml:lang="en">specialization of conceptual component</rdfs:label>
        <rdfs:subPropertyOf rdf:resource="https://w3id.org/OPLaX/hasRelatedConceptualComponent"/>
        <rdfs:range rdf:resource="https://w3id.org/OPLaX/ConceptualComponent"/>
        <rdfs:domain rdf:resource="https://w3id.org/OPLaX/ConceptualComponent"/>
    </owl:AnnotationProperty>
    


    <!-- https://w3id.org/OPLaX/specializationOfModule -->

    <owl:AnnotationProperty rdf:about="https://w3id.org/OPLaX/specializationOfModule">
        <rdfs:comment xml:lang="en">This property relates a Module to the Module it is a specialization of.</rdfs:comment>
        <rdfs:label xml:lang="en">specialization of module</rdfs:label>
        <rdfs:subPropertyOf rdf:resource="https://w3id.org/OPLaX/hasRelatedModule"/>
        <rdfs:range rdf:resource="https://w3id.org/OPLaX/Module"/>
        <rdfs:domain rdf:resource="https://w3id.org/OPLaX/Module"/>
        <owl:equivalentProperty rdf:resource="http://ontologydesignpatterns.org/opla-core/specializationOfModule"/>
    </owl:AnnotationProperty>
    


    <!-- https://w3id.org/OPLaX/specializationOfPattern -->

    <owl:AnnotationProperty rdf:about="https://w3id.org/OPLaX/specializationOfPattern">
        <rdfs:comment xml:lang="en">This property relates a Pattern to the Pattern it is a specialization of.</rdfs:comment>
        <rdfs:label xml:lang="en">specialization of pattern</rdfs:label>
        <rdfs:subPropertyOf rdf:resource="https://w3id.org/OPLaX/hasRelatedPattern"/>
        <rdfs:range rdf:resource="https://w3id.org/OPLaX/Pattern"/>
        <rdfs:domain rdf:resource="https://w3id.org/OPLaX/Pattern"/>
        <owl:equivalentProperty rdf:resource="http://ontologydesignpatterns.org/opla-core/specializationOfPattern"/>
    </owl:AnnotationProperty>
    


    <!-- 
    ///////////////////////////////////////////////////////////////////////////////////////
    //
    // Classes
    //
    ///////////////////////////////////////////////////////////////////////////////////////
     -->

    


    <!-- https://w3id.org/OPLaX/Axiom -->

    <owl:Class rdf:about="https://w3id.org/OPLaX/Axiom">
        <rdfs:subClassOf rdf:resource="https://w3id.org/OPLaX/OntologicalEntity"/>
        <rdfs:comment xml:lang="en">This class represents an axiom.</rdfs:comment>
        <rdfs:label xml:lang="en">Axiom</rdfs:label>
        <owl:equivalentClass rdf:resource="http://ontologydesignpatterns.org/opla-core/Axiom"/>
    </owl:Class>
    


    <!-- https://w3id.org/OPLaX/Class -->

    <owl:Class rdf:about="https://w3id.org/OPLaX/Class">
        <rdfs:subClassOf rdf:resource="https://w3id.org/OPLaX/OntologicalEntity"/>
        <rdfs:comment xml:lang="en">This class represents a class.</rdfs:comment>
        <rdfs:label xml:lang="en">Class</rdfs:label>
        <owl:equivalentClass rdf:resource="http://ontologydesignpatterns.org/opla-core/Class"/>
    </owl:Class>
    


    <!-- https://w3id.org/OPLaX/ConceptualComponent -->

    <owl:Class rdf:about="https://w3id.org/OPLaX/ConceptualComponent">
        <rdfs:comment xml:lang="en">This class represents a Conceptual Component, which is a complex structure often expressing a relational meaning (e.g., membership, locating). A conceptual component is the intensional counterpart of OWL implementations in ontologies (as sets of related predicates, classes and properties, and axioms). For example, an ontology may implement the membership component as an object property hasMember between a class Collection and a class Object, while another ontology may implement it as a n-ary relation class Membership connected to 3 arguments e.g., Collection, Time and Object. The conceptual components of an ontology indicate which types of facts, rather than which types of entities, an ontology can represent. The corresponding ODPs of a conceptual component show the adopted modelling solutions. This notion is inspired by the concept of Knowledge Pattern presented in Aldo Gangemi and Valentina Presutti, Towards a pattern science for the Semantic Web, SWJ, 2010.</rdfs:comment>
        <rdfs:label xml:lang="en">Conceptual Component</rdfs:label>
    </owl:Class>
    


    <!-- https://w3id.org/OPLaX/Domain -->

    <owl:Class rdf:about="https://w3id.org/OPLaX/Domain">
        <rdfs:comment xml:lang="en">This class represents a domain, an area of interest.</rdfs:comment>
        <rdfs:label xml:lang="en">Domain</rdfs:label>
    </owl:Class>
    


    <!-- https://w3id.org/OPLaX/Individual -->

    <owl:Class rdf:about="https://w3id.org/OPLaX/Individual">
        <rdfs:subClassOf rdf:resource="https://w3id.org/OPLaX/OntologicalEntity"/>
        <rdfs:comment xml:lang="en">This class represents an individual.</rdfs:comment>
        <rdfs:label xml:lang="en">Individual</rdfs:label>
        <owl:equivalentClass rdf:resource="http://ontologydesignpatterns.org/opla-core/Individual"/>
    </owl:Class>
    


    <!-- https://w3id.org/OPLaX/Module -->

    <owl:Class rdf:about="https://w3id.org/OPLaX/Module">
        <rdfs:subClassOf rdf:resource="https://w3id.org/OPLaX/OntologicalCollection"/>
        <rdfs:comment xml:lang="en">This class represents a module.</rdfs:comment>
        <rdfs:label xml:lang="en">Module</rdfs:label>
        <owl:equivalentClass rdf:resource="http://ontologydesignpatterns.org/opla-core/Module"/>
    </owl:Class>
    


    <!-- https://w3id.org/OPLaX/OntologicalCollection -->

    <owl:Class rdf:about="https://w3id.org/OPLaX/OntologicalCollection">
        <rdfs:comment xml:lang="en">This class represents an ontological collection, that is a collection of classes, properties, axioms, individuals formally defined.</rdfs:comment>
        <rdfs:label xml:lang="en">Ontological Collection</rdfs:label>
        <owl:equivalentClass rdf:resource="http://ontologydesignpatterns.org/opla-core/OntologicalCollection"/>
    </owl:Class>
    


    <!-- https://w3id.org/OPLaX/OntologicalEntity -->

    <owl:Class rdf:about="https://w3id.org/OPLaX/OntologicalEntity">
        <rdfs:comment xml:lang="en">This class represents an ontological entity, that is an axiom, class, individual or property defined in an ontological collection.</rdfs:comment>
        <rdfs:label xml:lang="en">Ontological Entity</rdfs:label>
        <owl:equivalentClass rdf:resource="http://ontologydesignpatterns.org/opla-core/OntologicalEntity"/>
    </owl:Class>
    


    <!-- https://w3id.org/OPLaX/Ontology -->

    <owl:Class rdf:about="https://w3id.org/OPLaX/Ontology">
        <rdfs:subClassOf rdf:resource="https://w3id.org/OPLaX/OntologicalCollection"/>
        <rdfs:comment xml:lang="en">This class represents an ontology.</rdfs:comment>
        <rdfs:label xml:lang="en">Ontology</rdfs:label>
        <owl:equivalentClass rdf:resource="http://ontologydesignpatterns.org/opla-core/Ontology"/>
    </owl:Class>
    


    <!-- https://w3id.org/OPLaX/Pattern -->

    <owl:Class rdf:about="https://w3id.org/OPLaX/Pattern">
        <rdfs:subClassOf rdf:resource="https://w3id.org/OPLaX/OntologicalCollection"/>
        <rdfs:comment xml:lang="en">This class represents a pattern.</rdfs:comment>
        <rdfs:label xml:lang="en">Pattern</rdfs:label>
        <owl:equivalentClass rdf:resource="http://ontologydesignpatterns.org/opla-core/Pattern"/>
    </owl:Class>
    


    <!-- https://w3id.org/OPLaX/PatternInstance -->

    <owl:Class rdf:about="https://w3id.org/OPLaX/PatternInstance">
        <rdfs:comment xml:lang="en">This class represents an instance of a pattern, that is the set of individuals that instantiate the ontology elements defined by a pattern.</rdfs:comment>
        <rdfs:label xml:lang="en">Pattern Instance</rdfs:label>
    </owl:Class>
    


    <!-- https://w3id.org/OPLaX/Property -->

    <owl:Class rdf:about="https://w3id.org/OPLaX/Property">
        <rdfs:subClassOf rdf:resource="https://w3id.org/OPLaX/OntologicalEntity"/>
        <rdfs:comment xml:lang="en">This class represents a property (object, datatype, annotation).</rdfs:comment>
        <rdfs:label xml:lang="en">Property</rdfs:label>
        <owl:equivalentClass rdf:resource="http://ontologydesignpatterns.org/opla-core/Property"/>
    </owl:Class>
    


    <!-- 
    ///////////////////////////////////////////////////////////////////////////////////////
    //
    // Individuals
    //
    ///////////////////////////////////////////////////////////////////////////////////////
     -->

    


    <!-- https://w3id.org/OPLaX/externalClass -->

    <owl:NamedIndividual rdf:about="https://w3id.org/OPLaX/externalClass">
        <rdfs:label xml:lang="en">external class</rdfs:label>
    </owl:NamedIndividual>
    


    <!-- https://w3id.org/OPLaX/externalIndividual -->

    <owl:NamedIndividual rdf:about="https://w3id.org/OPLaX/externalIndividual">
        <rdfs:label xml:lang="en">external individual</rdfs:label>
    </owl:NamedIndividual>
    


    <!-- https://w3id.org/OPLaX/externalPattern -->

    <owl:NamedIndividual rdf:about="https://w3id.org/OPLaX/externalPattern">
        <rdfs:label xml:lang="en">external pattern</rdfs:label>
    </owl:NamedIndividual>
    


    <!-- https://w3id.org/OPLaX/externalProperty -->

    <owl:NamedIndividual rdf:about="https://w3id.org/OPLaX/externalProperty">
        <rdfs:label xml:lang="en">external property</rdfs:label>
    </owl:NamedIndividual>
</rdf:RDF>



<!-- Generated by the OWL API (version 4.5.9.2019-02-01T07:24:44Z) https://github.com/owlcs/owlapi -->

